>[!lemma] Lemma 5.1.1 ([[../../../PDFs/howell2016.pdf#page=188|Source]])
>If $\gamma$ is any nonzero number, and $M$ and $N$ are any two integers with $M < N$, then
>$$\sum_{k=M}^N e^{-ik\gamma x}= \frac{e^{-iM \lambda x}-e^{-i(N+1)\gamma x}}{1-e^{-i \gamma x}}$$
>whenever $\gamma x$ is not an integral multiple of $2\pi$
>>[!proof]- Proof (started but unfinished)
>>$$\begin{align}
>> \sum_{k=M}^N e^{-ik\gamma x} &= e^{-iM\gamma x} + e^{-i(M+1)\gamma x} +e^{-i(M+2)\gamma x}+\dots+e^{-iN\gamma x} \\
>> &= e^{-iM\gamma x} \underbrace{ \big(1+ e^{-i\gamma x} + e^{-i2\gamma x} +\dots+e^{-i(N-M)\gamma x} \big) }_{ \text{geometric series} } \tag{1}
>>\end{align}$$
>>We identify a [[../Calculus/Series#^91927f|geometric series]] with $a=1$ and $r=e^{ix}$. Further, the condition $\lvert r \rvert \leq 1$ holds
>>$$\begin{align}
>> \lvert e^{-ix} \rvert &= \lvert \cos(-x)+i\sin(-x) \rvert \\
>> &=  \sqrt{ \cos^2(-x) + \sin^2(-x)} \\
>> &= 1 \tag{Pythagorean Identity}
>>\end{align}$$
>>therefore we can apply the convergence term from the [[../Calculus/Series#^91927f|geometric series]]
>>$$1+ e^{-i\gamma x} + e^{-i2\gamma x} +\dots+e^{-i(N-M)\gamma x} = \frac{1}{1-e^{-i\gamma x}}$$
>>We insert this result into equation $(1)$ and get
>>$$\begin{align}
>> \sum_{k=M}^N e^{-ik\gamma x} &= e^{-iM\gamma x} \big(1+ e^{-i\gamma x} + e^{-i2\gamma x} +\dots+e^{-i(N-M)\gamma x} \big) \\
>> &= e^{-iM\gamma x}\frac{1}{1-e^{i\gamma x}}
>>\end{align}$$
^bb8104

>[!lemma] Lemma 5.1.2 ([[../../../PDFs/howell2016.pdf#page=188|Source]])
>Let $p>0$ and let $M$ and $N$ be integers with $M < 0 < N$, then letting $\gamma=\frac{2\pi}{p}$
>$$\int _{-p/2}^{p/2} \left[ \sum_{k=M}^N e^{-ik \gamma x} \right] \, dx =p$$
>and
>$$\int _{-p/2}^{0} \left[ \sum_{k=-N}^N e^{ik\gamma x}\right] \, dx = \int _{0}^{p/2} \left[ \sum_{k=-N}^N e^{ik\gamma x}\right] \, dx = p$$
>
>>[!proof] Proof omitted

^183106

>[!lemma] Lemma (Riemann-Lebesgue Lemma) ([[../../../PDFs/howell2016.pdf#page=188|Source]])
>Let $p>0$ and assume $g$ is a piecewise continuous function on the interval $\left( -\frac{p}{2}, \frac{p}{2} \right)$. Then, letting $\gamma=\frac{2\pi}{p}$
>$$\lim_{ \substack{K \to \pm\infty\\K \in \mathbb{Z}} } \int _{-p/2}^{p/2} g(x)e^{-iK\gamma x} \, dx  =0$$
>>[!remark]
>>This lemma considers $g \in L^1$
>
>>[!proof]-
>>Denote the set $S$ and $E \subseteq S$ and the characteristic function $\chi$ of $E$ as 
>>$$\chi_{E}(x)=\begin{cases}
>> 1 &  x \in E \\
>> 0 & x \in \overline{E}
>>\end{cases}$$ 
>>Now, let $E=\left( -\frac{p}{2}, \frac{p}{2} \right) = (a,b)\subset \mathbb{R}$, then we can formulate the following integral as follows
>>$$\begin{align}
>> \int \chi_{\left( a, b \right)}(x)e^{iK\gamma x} \, dx &= \int _{a}^{b} e^{iK \gamma x} \, dx   \\
>> &= \frac{e^{iKb}-e^{iKa}}{iK}
>>\end{align}$$
>>As $K \to \infty$ we get
>>$$\begin{align} 
>> \lim_{ K \to \infty }  \frac{e^{iKb}-e^{iKa}}{iK} = 0 \tag{1}
>>\end{align}$$
>>More generally, given any function $f$ as a composition of characteristic functions, which is called a [simple function](https://proofwiki.org/wiki/Definition:Simple_Function), with $c_{n} \in \mathbb{R}$ and $a_{i} \leq b_{i} \in \mathbb{R}$ we can state for 
>>$$f = \sum_{n=1}^N c_{n}\chi(a_{i},b_{i})$$
>>that
>>$$\lim_{ K \to \infty } \int f(x)e^{iKx} \, dx =0 \tag{2} $$
>>as a result of equation $(1)$
>>>[!note]- Note on Simple Functions and Density in $\mathcal{L}^p$
>>>Let $\mathcal{E}(\Sigma)$ be the space of simple functions which can be described as a composition of characteristic functions and $\mathcal{L}^p$ the space of $p$-integrable functions, then the space of simple functions $\mathcal{E} \cap \mathcal{L}^p$ is dense in $\mathcal{L}^p$ [(Source)](https://proofwiki.org/wiki/Space_of_Simple_P-Integrable_Functions_is_Everywhere_Dense_in_Lebesgue_Space)
>>
>>Now, let $f \in \mathcal{L}^1$ be arbitrary and $\varepsilon>0$. Since the space of simple functions $\mathcal{E}(\Sigma)$ is dense in $\mathcal{L}^1$ we know that we can find some $g \in \mathcal{E}(\Sigma) \cap \mathcal{L}^1$ such that
>>$$\int  \lvert f-g \rvert  \, dx < \varepsilon \tag{3}$$
>>Since $g$ is a simple function we know by our result in equation $(2)$ that for any $\varepsilon>0$ we can find an $N$ such that for all $K>N$
>>$$\int \lvert g(x)e^{iKx} \rvert  \, dx < \varepsilon \tag{4}$$
>>Using the additivity property we can easily do the following expansion
>>$$\begin{align}
>>\int  f(x)e^{iKx}  \, dx &= \int  f(x)e^{iKx}  -g(x)e^{iKx} + g(x)e^{iKx} \,dx  \\
>> &= \int  \Big(f(x)-g(x)\Big)  e^{iKx} + g(x)e^{iKx} \,dx \\
>> &= \int  \Big(f(x)-g(x)\Big)  e^{iKx} \, dx + \int  g(x)e^{iKx} \,dx \tag{5}
>>\end{align}$$
>>Now we can do the following, taking the absolute value of 
>>$$\begin{align}
>>\left\lvert   \int  f(x)e^{iKx}  \, dx  \right\rvert &= \left\lvert  \int  \Big(f(x)-g(x)\Big)  e^{iKx} \, dx + \int  g(x)e^{iKx} \,dx    \right\rvert \tag{Result (5)} \\
>> &\leq \left\lvert  \int  \Big(f(x)-g(x)\Big)  e^{iKx} \, dx \right\rvert + \left\lvert  \int  g(x)e^{iKx} \,dx      \right\rvert \tag{TI}\\
>> &\leq   \int\Bigg\lvert  \Big(f(x)-g(x)\Big)  e^{iKx} \Bigg\rvert\, dx  + \left\lvert  \int  g(x)e^{iKx} \,dx      \right\rvert \tag{Absolute Value Int.}\\
>> &=   \int\Bigg\lvert  \Big(f(x)-g(x)\Big)\Bigg\lvert\;\underbrace{ \Bigg\lvert  e^{iKx} \Bigg\rvert }_{ =1 }\, dx  + \left\lvert  \int  g(x)e^{iKx} \,dx      \right\rvert \\
>> &=   \underbrace{ \int\Bigg\lvert  \Big(f(x)-g(x)\Big)\Bigg\lvert\;\, dx }_{  \substack{<\varepsilon \\ \text{ by $(3)$}}  }  + \underbrace{ \left\lvert  \int  g(x)e^{iKx} \,dx      \right\rvert }_{ \substack{<\varepsilon \\ \text{ by $(4)$}} } \\
>> &< 2\varepsilon
>>\end{align}$$
>>Since $\varepsilon$ can be chosen arbitrarily small, we can always find a $N\in\mathbb{N}$ such that $K>N$ fulfills the result. Therefore
>>$$\lim_{ K \to \infty } \int f(x)e^{iKx} \, dx =0 \tag*{$\square$} $$

^e3e352

>[!def] Definition Dirichlet Kernel ([[../../../PDFs/howell2016.pdf#page=189|Source]])
>Let $p> 0$ and let $M, N \in \mathbb{Z}$ with $M<N$. The corresponding Dirichlet Kernel is the function $D_{M,N}$ given by
>$$D_{M,N}(x)=\frac{1}{p}\sum_{k=M}^N e^{-2\pi \omega _{k}x}$$
>with $\omega_{k}=\frac{p}{k}$
>>[!remark]
>>We can define $\gamma=\frac{2\pi}{p}$ and get 
>>$$D_{M,N}(x)=\frac{1}{p}\sum_{k=M}^N e^{-2\pi \gamma x}$$


>[!remark] Remark on the Dirichlet Kernel and its Integration Properties
>[[#^bb8104|Lemma 5.1.1]] gives the following result
>$$D_{M,N}(x) = \frac{e^{-iM \gamma x}-e^{-i(N+1)\gamma x}}{p(1-e^{-i \gamma x})}$$
>Further, [[#^183106| Lemma 5.1.2]] gives
>$$\begin{align}
>\int _{-p / 2}^{p/2} D_{M,N}(x) \, dx &= \int _{-p / 2}^{p/2} \frac{e^{-iM \gamma x}-e^{-i(N+1)\gamma x}}{p(1-e^{-i \gamma x})} \, dx \\
> &= \frac{1}{p}\int _{-p / 2}^{p/2} \frac{e^{-iM \gamma x}-e^{-i(N+1)\gamma x}}{1-e^{-i \gamma x}} \, dx\\
> &= \frac{1}{p}p\\
> &= 1
>\end{align} $$
>and similarly
>$$\int _{-p / 2}^{0} D_{-N,N}(x) \, dx = \int _{0}^{p/2} D_{-N,N}(x) \, dx = \frac{1}{2}$$

^303c05

>[!Lemma] Lemma Representation of Fourier Coefficients with Dirichlet Kernel ([[../../../PDFs/howell2016.pdf#page=189|Source]])
>Denote the Fourier series 
>$$\mathcal{F}[f]|_{t} = \sum_{k=-\infty}^\infty c_{k}e^{i 2\pi \omega_{k}t}$$
>then for some $t_{0} \in (-\frac{p}{2}, \frac{p}{2})$
>$$\sum_{k=M}^N c_{k}e^{i 2\pi \omega_{k} t_{0}}= \int _{-p/2}^{p/2} f(t_{0}+x)D_{M,N}(x) \, dx $$
>>[!proof]-
>> Using the definition the [[4 - Complex Exponential Fourier Series#^cc2d06| Fourier coefficients]] at $t_0$ we get
>> $$\begin{align}
>>c_{k}e^{i 2 \pi \omega_{k}t_{0}}&= \left(\frac{1}{p}\int _{t_{0}-p / 2}^{t_{0}+p / 2} f(\tau)e^{-i2\pi \omega_{k}\tau}\, d\tau \right)e^{i2\pi \omega k t_{0}} \\
>> &= \frac{1}{p}\int _{t_{0}-p / 2}^{t_{0}+p / 2} f(\tau)e^{-i2\pi \omega_{k}(\tau-t_{0})}\, d\tau \\
>> &= \frac{1}{p}\int _{-p / 2}^{p / 2} f(t_{0}+x)e^{-i2\pi \omega_{k}x}\, dx \tag{$x = \tau-t_{0}$}\\
>>\end{align}$$
>> Expanding on the sum gives
>> $$\begin{align}
>> \sum_{k=M}^N c_{k}e^{i 2\pi \omega_{k} t_{0}} &= \sum_{k=M}^N \frac{1}{p}\int _{-p / 2}^{p / 2} f(t_{0}+x)e^{-i2\pi \omega_{k}x}\, dx \\
>> &=  \int _{-p / 2}^{p / 2} \frac{1}{p} \sum_{k=M}^N  f(t_{0}+x)e^{-i2\pi \omega_{k}x}\, dx \\
>> &=  \int _{-p / 2}^{p / 2}  f(t_{0}+x)\underbrace{ \left(\frac{1}{p}\sum_{k=M}^N  e^{-i2\pi \omega_{k}x}\right) }_{ =D_{M,N}(x) }\, dx \\ 
>>&=  \int _{-p / 2}^{p / 2}  f(t_{0}+x)D_{M,N}(x)\, dx \tag*{$\square$}\\
>>\end{align}$$
>>>[!note]
>>>1. In the first line we shifted the integration interval by $t_0$ while preserving the period of the periodic function
>>>2. The change of variable makes the term $t_0$ vanish in the integration bounds in the last line of the first paragraph

^8c3eb2

>[!lemma] Lemma 5.1.3 ([[../../../PDFs/howell2016.pdf#page=190|Source]])
>Let $f$ be a periodic, piecewise continuous function with
>$$\mathcal{F}[t]|_{t}= \sum_{k=-\infty}^\infty c_{k}e^{i 2 \pi \omega_{k}t}$$
>Let $t_{0}$ be any point on the real line at which $f(t)$ is continuous. Then for any pair  $M,N \in \mathbb{Z}$ with $M<0<N$
>$$\sum_{k=M}^N c_{k}e^{i 2 \pi \omega_{k}t_{0}}= \int _{-p / 2}^{p / 2}  \Big(f(t_{0}+x)-f(t_{0})\Big)D_{M,N}(x)\, dx +f(t_{0})$$ 
>>[!proof]-
>>Denote
>>$$\begin{align}
>> f_{0}^- &= \lim_{ x \to 0^- } f(t_{0}+x) \\ 
>> f_{0}^+ &= \lim_{ x \to 0^+ } f(t_{0}+x)  
>>\end{align}$$
>>and 
>>$$f_{0}(x) = \begin{cases}
>> f_{0}^- &  \text{ if } x < 0 \\
>> f_{0}^+ & \text{ if } > 0 
>>\end{cases}\tag{1}$$
>>We make use of the [[#^8c3eb2| Dirichlet kernel representation lemma]]. 
>>$$\begin{align}
>> \sum_{k=M}^N c_{k}e^{i 2 \pi \omega_{k}t_{0}} &= \int _{-p/2}^{p/2} f(t_{0}+x)D_{M,N}(x) \, dx  \\
>> &= \int _{-p/2}^{p/2} \Big(f(t_{0}+x) +f_{0}(x)-f_{0}(x)\Big)D_{M,N}(x) \, dx \\
>> &= \int _{-p/2}^{p/2} \Big(f(t_{0}+x) +f_{0}(x)\Big)D_{M,N}(x) \, dx  - \int_{-p/2}^{p/2} f_{0}(x)D_{M,N}(x) \, dx 
>>\end{align}$$
>>Note, we assume $f$ is continuous at $t_0$, therefore we have the identity
>>$$f^-_{0} = f(t_{0})= f^+_{0}$$
>>Thus, $f_{0}(x)=f(t_{0})$ as can be easily seen from equation $(1)$, therefore we get
>>$$\begin{align}
>> \phantom{\sum_{k=M}^N c_{k}e^{i 2 \pi \omega_{k}t_{0}}} &= \int _{-p/2}^{p/2} \Big(f(t_{0}+x) +f(t_{0})\Big)D_{M,N}(x) \, dx  - f(t_{0})\underbrace{ \int_{-p/2}^{p/2} D_{M,N}(x)U \, dx }_{ =1 } \;  \tag{Dirichlet Int.}\\
>> &= \int _{-p/2}^{p/2} \Big(f(t_{0}+x) +f(t_{0})\Big)D_{M,N}(x) \, dx  - f(t_{0}) \tag*{$\square$}
>>\end{align}$$
>>>[!note]
>>>For the final result we used the [[#^303c05| Dirichlet kernel integration properties]].

^ce82c1


>[!lemma] Lemma 5.1.4 ([[../../../PDFs/howell2016.pdf#page=190|Source]])
>Let $f$ be a periodic, piecewise continuous function with
>$$\mathcal{F}[t]|_{t}= \sum_{k=-\infty}^\infty c_{k}e^{i 2 \pi \omega_{k}t}$$
>Let $t_{0}$ be any point on the real line and let $f_{0}^-$ and $f_{0}⁺$ be the values
>$$\begin{align}
> f_{0}^- &= \lim_{ x \to 0^- } f(t_{0}+x) \\ 
> f_{0}^+ &= \lim_{ x \to 0^+ } f(t_{0}+x)  
>\end{align}$$
>Then, for any positive integer $N$
>$$\sum_{k=M}^N c_{k}e^{i 2 \pi \omega_{k}t_{0}}= \int _{-p / 2}^{p / 2}  \Big(f(t_{0}+x)-f_{0}(x)\Big)D_{-N,N}(x)\, dx + \frac{1}{2}(f_{0}^- + f_{0}^+)$$
>where
>$$f_{0}(x) = \begin{cases}
> f_{0}^- &  \text{ if } x < 0 \\
> f_{0}^+ & \text{ if } > 0 
>\end{cases}$$
>>[!pic]- Illustration
>>![[figures/5_1_proof_prelim.png|center]]
>
>>[!proof]-
>>Note, we have $M=-N$, therefore we start with
>>$$\begin{align}
>>\sum_{k=M}^N c_{k}e^{i 2 \pi \omega_{k}t_{0}}&= \int _{-p/2}^{p/2} f(t_{0}+x)D_{-N,N}(x) \, dx \\
>> &=\int _{-p/2}^{p/2} \Big( f(t_{0}+x) - f_{0}(x) + f_{0}(x)\Big)D_{-N,N}(x) \, dx  \\
>> &=\int _{-p/2}^{p/2} \Big( f(t_{0}+x) - f_{0}(x)\Big) D_{-N,N}(x) \, dx + \int _{-p/2}^{p/2}f_{0}(x)D_{-N,N}(x)
>>\end{align}$$
>>Further note, we can split the second integral at $0$ into its upper and lower part. Additionally, we make use of the definition of $f_0$ while splitting the integral and the [[#^303c05|integration properties of the Dirichlet kernel]], we get
>>$$\begin{align}
>>&= \int _{-p/2}^{p/2} \Big( f(t_{0}+x) - f_{0}(x)\Big) D_{-N,N}(x) \, dx + \underbrace{ \int _{-p/2}^{0}f_{0}^-D_{-N,N}(x) + \int _{0}^{p/2}f_{0}^+D_{-N,N}(x) }_{ = \int _{-p/2}^{p/2}f_{0}(x)D_{-N,N}(x)}\\
>>&= \int _{-p/2}^{p/2} \Big( f(t_{0}+x) - f_{0}(x)\Big) D_{-N,N}(x) \, dx +  f_{0}^-\underbrace{ \int _{-p/2}^{0}D_{-N,N}(x) }_{ =\frac{1}{2} } + f_{0}^+\underbrace{ \int _{0}^{p/2}D_{-N,N}(x)  }_{ =\frac{1}{2} } \\
>>&=\int _{-p/2}^{p/2} \Big( f(t_{0}+x) - f_{0}(x)\Big) D_{-N,N}(x) \, dx + \frac{1}{2}(f_{0}^- + f_{0}^+) \tag*{$\square$}
>>\end{align}$$

^fa5a3e
