>[!lemma] Proposition ([[../../../../PDFs/judson2022.pdf#page=204|Source]])
>Let $R$ be a ring with $a,b \in R$, then
>1. $a0=0a=0$
>2. $a(-b)=(-a)b=-ab$
>3. $(-a)(-b)=ab$
>
>>[!proof]-
>>1. $\,$ $$a0=a(0+0)=a0 + \underbrace{ a0 }_{ =0 }$$
>>Hence $a0=0$. The direction for $0a$ works similarly.
>>
>>2. We want to show that $a(-b)+ab = 0$  $$ab + a(-b)=a(b-b)=a 0=0$$
>>3. Follows from (2)
>>$$(-a)(-b)=-(a(-b))=-(-ab)= ab \tag*{$\square$}$$

>[!def] Definition Subring ([[../../../../PDFs/judson2022.pdf#page=205|Source]])
>Let $R$ be a ring. Then $S$ is a **<span style="color:#38ffa9">subring</span>** if
>1. $S \subset R$
>2. $S$ is a [[1 - Algebraic Structures#^2c4055|ring]] under the inherited operations from $R$